\documentclass[a4paper,10pt]{article}

\usepackage{amstex}

% latex file for automatic generation of formulas
% lines beginning with %% will be used for image names
% put each formula in an extra eqnarray* environement
% first line contains the actual formulas
% the second line is for the order of the parameters

\begin{document}

\begin{eqnarray*}
%% lj
V(r)=4\epsilon\left[\left(\frac{\sigma}{r}\right)^{12}-\left(\frac{\sigma}{r}\right)^{6}\right]\\
\epsilon,\sigma
\end{eqnarray*}

\begin{eqnarray*}
%% morse
V(r)=D_e ( 1-e^{-a(r-r_0)} )^2 \\
D_e,a,r_0
\end{eqnarray*}

\begin{eqnarray*}
%% softshell
V(r)=\left(\frac{\alpha}{r}\right)^\beta \\
\alpha,\beta
\end{eqnarray*}

\begin{eqnarray*}
%% power_decay
V(r)=\alpha\left(\frac{1}{r}\right)^\beta \\
\alpha,\beta
\end{eqnarray*}

\begin{eqnarray*}
%% exp_decay
V(r)=\alpha \exp\left(-\beta r\right) \\
\alpha,\beta
\end{eqnarray*}

\begin{eqnarray*}
%% eopp
V(r)=\frac{C_1}{r^{\eta_1}}+\frac{C_2}{r^{\eta_2}}\cos\left(kr+\varphi\right) \\
C_1,\eta_1,C_2,\eta_2,k,\varphi
\end{eqnarray*}

\begin{eqnarray*}
%% eopp_exp
V(r)=C_1\exp\left(-\eta_1r\right)+\frac{C_2}{r^{\eta_2}}\cos\left(kr+\varphi\right) \\
C_1,\eta_1,C_2,\eta_2,k,\varphi
\end{eqnarray*}

\begin{eqnarray*}
%% meopp
V(r)=\frac{C_1}{\left(r-r_0\right)^{\eta_1}}+\frac{C_2}{r^{\eta_2}}\cos\left(kr+\varphi\right) \\
C_1,\eta_1,C_2,\eta_2,k,\varphi, r_0
\end{eqnarray*}

\begin{eqnarray*}
%% universal
F(n)=F_0\left[\frac{q}{q-p}n^p-\frac{p}{q-p}n^q\right]+F_1n \\
F_0,p,q,F_1
\end{eqnarray*}

\begin{eqnarray*}
%% pohlong
F(n)=F_0\left[1-\gamma\ln n\right]n^\gamma \\
F_0,\gamma
\end{eqnarray*}

\begin{eqnarray*}
%% parabola
\rho(r)=ar^2+br+c \\
a,b,c
\end{eqnarray*}

\begin{eqnarray*}
%% csw
\rho(r)=\frac{1+a_1\cos\left(\alpha r\right)+a_2\sin\left(\alpha r\right)}{r^\beta} \\
a_1,a_2,\alpha,\beta
\end{eqnarray*}

\begin{eqnarray*}
%% ms
V(r)=D_e (e^{a*(1-\frac{r}{r_0})}-2e^{a(1-\frac{r}{r_0})/2}) \\
D_e,a,r_0
\end{eqnarray*}

\begin{eqnarray*}
%% const
V(r)= c \\
c
\end{eqnarray*}

\begin{eqnarray*}
%% sqrt
V(r)= \alpha \sqrt{r/\beta} \\
\alpha,\beta
\end{eqnarray*}

\begin{eqnarray*}
%% mexp_decay
V(r)=\alpha e^{-\beta(r-r_0)} \\
\alpha,\beta,r_0
\end{eqnarray*}

\begin{eqnarray*}
%% strmm
V(r)= 2\alpha e^{-\beta/2(r-r_0)} - \gamma ( 1+ \delta (r-r_0)e^{-\delta (r-r_0)}) \\
\alpha,\beta,\gamma,\delta,r_0
\end{eqnarray*}

\end{document}
